src/Framework/CheckingAnnotate.v
@@ -1445,7 +1445,6 @@ Section Top.
               end
 
         | AS.Vfun f1 ρ1 xs1 e1, AT.Vfun f2 ρ2 xs2 e2 =>
-            (* note function arguments and result are always exposed regardless of whether a function is known or unknown *)
             length xs1 = length xs2 /\
               match i with
               | 0 => True
@@ -1604,12 +1603,11 @@ Section Top.
   Lemma trans_correct_top_approx W1 W2 e1 e2 :
     leq W1 W2 ->
     trans_correct_top W1 e1 e2 ->
-    trans_correct_top W2 e1 e2.
+    exists e2', trans_correct_top W2 e1 e2'.
   Proof.
     unfold trans_correct_top.
     intros HW HT.
     destruct HT as [e2' HT'].
-    split; auto; intros.
   Abort.
 
 End Top.
